<rdf:RDF xmlns="https://example.com/semshift#"
     xml:base="https://example.com/semshift"
     xmlns:cc="http://creativecommons.org/ns#"
     xmlns:owl="http://www.w3.org/2002/07/owl#"
     xmlns:rdf="http://www.w3.org/1999/02/22-rdf-syntax-ns#"
     xmlns:rdfs="http://www.w3.org/2000/01/rdf-schema#"
     xmlns:xml="http://www.w3.org/XML/1998/namespace"
     xmlns:vann="http://purl.org/vocab/vann/"
     xmlns:dcterms="http://purl.org/dc/terms/"
     xmlns:semshift="https://example.com/semshift#">
    <owl:Ontology rdf:about="https://example.com/semshift#">
        <cc:license rdf:resource="https://creativecommons.org/publicdomain/zero/1.0"/>
        <dcterms:creator>Sabine Tittel</dcterms:creator>
        <dcterms:description xml:lang="en">A model for the representation of methods of semantic shift -- SemShift.</dcterms:description>
        <dcterms:rights>CC-Zero</dcterms:rights>
        <dcterms:title xml:lang="en">Model for Semantic Shift Methods</dcterms:title>
        <vann:preferredNamespacePrefix>semshift</vann:preferredNamespacePrefix>
        <vann:preferredNamespaceUri rdf:resource="https://example.com/semshift#"/>
        <owl:versionInfo rdf:datatype="http://www.w3.org/2001/XMLSchema#decimal">1.0</owl:versionInfo>
    </owl:Ontology>

<!--
///////////////////////////////////////////////////////////////////////////////////////
//
// Annotation properties
//
///////////////////////////////////////////////////////////////////////////////////////
 -->

<!-- http://creativecommons.org/ns#license -->

<owl:AnnotationProperty rdf:about="http://creativecommons.org/ns#license"/>

<!-- http://purl.org/dc/elements/1.1/date -->

<owl:AnnotationProperty rdf:about="http://purl.org/dc/elements/1.1/date"/>

<!-- http://purl.org/dc/elements/1.1/description -->

<owl:AnnotationProperty rdf:about="http://purl.org/dc/elements/1.1/description"/>

<!-- http://purl.org/dc/elements/1.1/title -->

<owl:AnnotationProperty rdf:about="http://purl.org/dc/elements/1.1/title"/>

<!-- http://purl.org/dc/terms/creator -->

<owl:AnnotationProperty rdf:about="http://purl.org/dc/terms/creator"/>

<!-- http://purl.org/dc/terms/description -->

<owl:AnnotationProperty rdf:about="http://purl.org/dc/terms/description"/>

<!-- http://purl.org/dc/terms/issued -->

<owl:AnnotationProperty rdf:about="http://purl.org/dc/terms/issued"/>

<!-- http://purl.org/dc/terms/language -->

<owl:AnnotationProperty rdf:about="http://purl.org/dc/terms/language"/>

<!-- http://purl.org/dc/terms/rights -->

<owl:AnnotationProperty rdf:about="http://purl.org/dc/terms/rights"/>

<!-- http://purl.org/dc/terms/title -->

<owl:AnnotationProperty rdf:about="http://purl.org/dc/terms/title"/>

<!-- http://purl.org/vocab/vann/preferredNamespacePrefix -->

<owl:AnnotationProperty rdf:about="http://purl.org/vocab/vann/preferredNamespacePrefix"/>

<!-- http://purl.org/vocab/vann/preferredNamespaceUri -->

<owl:AnnotationProperty rdf:about="http://purl.org/vocab/vann/preferredNamespaceUri"/>

<!-- http://www.w3.org/2002/07/owl#versionInfo -->

<owl:AnnotationProperty rdf:about="http://www.w3.org/2002/07/owl#versionInfo"/>

<!--
///////////////////////////////////////////////////////////////////////////////////////
//
// Object Properties
//
///////////////////////////////////////////////////////////////////////////////////////
-->

<!-- https://example.com/semshift#rhetoricalFigure -->

<owl:ObjectProperty rdf:about="https://https://example.com/semshift#rhetoricalFigure">
    <rdfs:domain rdf:resource="http://www.w3.org/ns/lemon/ontolex#LexicalSense"/>
    <rdfs:range  rdf:resource="http://www.w3.org/ns/lemon/ontolex#LexicalSense"/>
    <rdfs:subPropertyOf rdf:resource="http://www.w3.org/ns/lemon/vartrans#senseRel"/>
    <rdfs:comment xml:lang="en">The 'rhetoricalFigure' property indicates that the lexical sense of a linguistic sign represents a figure of speech with respect to the lexical sense of the linguistic sign referred to.</rdfs:comment>
    <rdfs:label xml:lang="en">is rhetorical figure of</rdfs:label>
    <rdfs:label xml:lang="en">is figure of speech of</rdfs:label>
    <rdfs:label xml:lang="fr">est une figure de style de</rdfs:label>
    <rdfs:label xml:lang="de">ist rethorische Stilfigur in Bezug auf</rdfs:label>
</owl:ObjectProperty>

<!-- https://example.com/semshift#metaphor -->

<owl:ObjectProperty rdf:about="https://https://example.com/semshift#metaphor">
    <rdfs:domain rdf:resource="http://www.w3.org/ns/lemon/ontolex#LexicalSense"/>
    <rdfs:range  rdf:resource="http://www.w3.org/ns/lemon/ontolex#LexicalSense"/>
    <rdfs:subPropertyOf rdf:resource="http://www.w3.org/ns/lemon/vartrans#senseRel"/>
    <rdfs:comment xml:lang="en">The 'metaphor' property indicates that the lexical sense of a linguistic sign represents a metaphor of the lexical sense of the linguistic sign referred to.</rdfs:comment>
    <rdfs:label xml:lang="en">is metaphor of</rdfs:label>
    <rdfs:label xml:lang="fr">est une métaphore de</rdfs:label>
    <rdfs:label xml:lang="de">ist Metapher von</rdfs:label>
</owl:ObjectProperty>

<!-- https://example.com/semshift#image -->

<owl:ObjectProperty rdf:about="https://https://example.com/semshift#image">
    <rdfs:domain rdf:resource="http://www.w3.org/ns/lemon/ontolex#LexicalSense"/>
    <rdfs:range  rdf:resource="http://www.w3.org/ns/lemon/ontolex#LexicalSense"/>
    <rdfs:subPropertyOf rdf:resource="http://www.w3.org/ns/lemon/vartrans#senseRel"/>
    <rdfs:comment xml:lang="en">The 'image' property indicates that the lexical sense of a linguistic sign represents an image (an extended metaphor) of the lexical sense of the linguistic sign referred to.</rdfs:comment>
    <rdfs:label xml:lang="en">uses within an image</rdfs:label>
    <rdfs:label xml:lang="fr">utilise dans une image</rdfs:label>
    <rdfs:label xml:lang="de">verwendet bildhaft</rdfs:label>
</owl:ObjectProperty>

<!-- https://example.com/semshift#allegory -->

<owl:ObjectProperty rdf:about="https://https://example.com/semshift#allegory">
    <rdfs:domain rdf:resource="http://www.w3.org/ns/lemon/ontolex#LexicalSense"/>
    <rdfs:range  rdf:resource="http://www.w3.org/ns/lemon/ontolex#LexicalSense"/>
    <rdfs:subPropertyOf rdf:resource="http://www.w3.org/ns/lemon/vartrans#senseRel"/>
    <rdfs:comment xml:lang="en">The 'allegory' property indicates that the lexical sense of a linguistic sign represents an allegory (an extended metaphor) of the lexical sense of the linguistic sign referred to.</rdfs:comment>
    <rdfs:label xml:lang="en">uses within an allegory</rdfs:label>
    <rdfs:label xml:lang="fr">utilise dans une allégorie</rdfs:label>
    <rdfs:label xml:lang="de">verwendet in einer Allegorie</rdfs:label>
</owl:ObjectProperty>

<!-- https://example.com/semshift#personification -->

<owl:ObjectProperty rdf:about="https://https://example.com/semshift#personification">
    <rdfs:domain rdf:resource="http://www.w3.org/ns/lemon/ontolex#LexicalSense"/>
    <rdfs:range  rdf:resource="http://www.w3.org/ns/lemon/ontolex#LexicalSense"/>
    <rdfs:subPropertyOf rdf:resource="http://www.w3.org/ns/lemon/vartrans#senseRel"/>
    <rdfs:comment xml:lang="en">The 'personification' property indicates that the lexical sense of a linguistic sign represents a personification (anthropomorphism, a specific kind of allegory and, thus, an extended metaphor) of the lexical sense of the linguistic sign referred to.</rdfs:comment>
    <rdfs:label xml:lang="en">is personification of</rdfs:label>
    <rdfs:label xml:lang="fr">est une personnification de</rdfs:label>
    <rdfs:label xml:lang="de">ist Personifizierung von</rdfs:label>
</owl:ObjectProperty>

<!-- https://example.com/semshift#comparison -->

<owl:ObjectProperty rdf:about="https://https://example.com/semshift#comparison">
    <rdfs:domain rdf:resource="http://www.w3.org/ns/lemon/ontolex#LexicalSense"/>
    <rdfs:range  rdf:resource="http://www.w3.org/ns/lemon/ontolex#LexicalSense"/>
    <rdfs:subPropertyOf rdf:resource="http://www.w3.org/ns/lemon/vartrans#senseRel"/>
    <rdfs:comment xml:lang="en">The 'comparison' property indicates that the lexical sense of a linguistic sign represents a comparison of the lexical sense of the linguistic sign referred to.</rdfs:comment>
    <rdfs:label xml:lang="en">uses as a comparison</rdfs:label>
    <rdfs:label xml:lang="fr">utilise dans une comparaison</rdfs:label>
    <rdfs:label xml:lang="de">verwendet als Vergleich</rdfs:label>
</owl:ObjectProperty>

<!-- https://example.com/semshift#metonymy -->

<owl:ObjectProperty rdf:about="https://https://example.com/semshift#metonymy">
    <rdfs:domain rdf:resource="http://www.w3.org/ns/lemon/ontolex#LexicalSense"/>
    <rdfs:range  rdf:resource="http://www.w3.org/ns/lemon/ontolex#LexicalSense"/>
    <rdfs:subPropertyOf rdf:resource="http://www.w3.org/ns/lemon/vartrans#senseRel"/>
    <rdfs:comment xml:lang="en">The 'metonymy' property indicates that the lexical sense of a linguistic sign represents a metonymy of the lexical sense of the linguistic sign referred to.</rdfs:comment>
    <rdfs:label xml:lang="en">is metonymy of</rdfs:label>
    <rdfs:label xml:lang="fr">est une métonymie de</rdfs:label>
    <rdfs:label xml:lang="de">ist Metonymie von</rdfs:label>
</owl:ObjectProperty>

<!-- https://example.com/semshift#synechdoche -->

<owl:ObjectProperty rdf:about="https://https://example.com/semshift#synechdoche">
    <rdfs:domain rdf:resource="http://www.w3.org/ns/lemon/ontolex#LexicalSense"/>
    <rdfs:range  rdf:resource="http://www.w3.org/ns/lemon/ontolex#LexicalSense"/>
    <rdfs:subPropertyOf rdf:resource="http://www.w3.org/ns/lemon/vartrans#senseRel"/>
    <owl:equivalentProperty>
        <owl:ObjectProperty rdf:about="http://www.lexinfo.net/ontology/3.0/lexinfo#meronymTerm"/>
    </owl:equivalentProperty>
    <rdfs:comment xml:lang="en">The 'synechdoche' property indicates that the lexical sense of a linguistic sign represents a synechdoche of the lexical sense of the linguistic sign referred to.</rdfs:comment>
    <rdfs:label xml:lang="en">is synechdoche of</rdfs:label>
    <rdfs:label xml:lang="fr">est une synecdoque de</rdfs:label>
    <rdfs:label xml:lang="de">ist Synekdoche von</rdfs:label>
</owl:ObjectProperty>

<!-- https://example.com/semshift#irony -->

<owl:ObjectProperty rdf:about="https://https://example.com/semshift#irony">
    <rdfs:domain rdf:resource="http://www.w3.org/ns/lemon/ontolex#LexicalSense"/>
    <rdfs:range  rdf:resource="http://www.w3.org/ns/lemon/ontolex#LexicalSense"/>
    <rdfs:subPropertyOf rdf:resource="http://www.w3.org/ns/lemon/vartrans#senseRel"/>
    <rdfs:comment xml:lang="en">The 'irony' property indicates that the lexical sense of a linguistic sign represents an irony (a kind of metonymie) of the lexical sense of the linguistic sign referred to.</rdfs:comment>
    <rdfs:label xml:lang="en">is ironic use of</rdfs:label>
    <rdfs:label xml:lang="fr">est une utilisation ironique de</rdfs:label>
    <rdfs:label xml:lang="de">ist ironische Verwendung von</rdfs:label>
</owl:ObjectProperty>

<!-- https://example.com/semshift#euphemism -->

<owl:ObjectProperty rdf:about="https://https://example.com/semshift#euphemism">
    <rdfs:domain rdf:resource="http://www.w3.org/ns/lemon/ontolex#LexicalSense"/>
    <rdfs:range  rdf:resource="http://www.w3.org/ns/lemon/ontolex#LexicalSense"/>
    <rdfs:subPropertyOf rdf:resource="http://www.w3.org/ns/lemon/vartrans#senseRel"/>
    <rdfs:comment xml:lang="en">The 'euphemism' property indicates that the lexical sense of a linguistic sign represents a euphemism (a specific kind of irony and, thus, of metonymy) of the lexical sense of the linguistic sign referred to.</rdfs:comment>
    <rdfs:label xml:lang="en">is euphemistic use of</rdfs:label>
    <rdfs:label xml:lang="fr">est une utilisation euphémique de</rdfs:label>
    <rdfs:label xml:lang="de">ist Euphemismus von</rdfs:label>
</owl:ObjectProperty>

<!-- https://example.com/semshift#salutation -->

<owl:ObjectProperty rdf:about="https://https://example.com/semshift#salutation">
    <rdfs:domain rdf:resource="http://www.w3.org/ns/lemon/ontolex#LexicalSense"/>
    <rdfs:range  rdf:resource="http://www.w3.org/ns/lemon/ontolex#LexicalSense"/>
    <rdfs:subPropertyOf rdf:resource="http://www.w3.org/ns/lemon/vartrans#senseRel"/>
    <rdfs:comment xml:lang="en">The 'salutation' property indicates that the lexical sense of a linguistic sign represents a salutation (a specific kind of metonymy) using the lexical sense of the linguistic sign referred to.</rdfs:comment>
    <rdfs:label xml:lang="en">uses as salutation</rdfs:label>
    <rdfs:label xml:lang="fr">utilise comme salutation</rdfs:label>
    <rdfs:label xml:lang="de">verwendet als Grußwort</rdfs:label>
</owl:ObjectProperty>

<!-- https://example.com/semshift#toponym -->

<owl:ObjectProperty rdf:about="https://https://example.com/semshift#toponym">
    <rdfs:domain rdf:resource="http://www.w3.org/ns/lemon/ontolex#LexicalSense"/>
    <rdfs:range  rdf:resource="http://www.w3.org/ns/lemon/ontolex#LexicalSense"/>
    <rdfs:subPropertyOf rdf:resource="http://www.w3.org/ns/lemon/vartrans#senseRel"/>
    <rdfs:comment xml:lang="en">The 'toponym' property indicates that the lexical sense of a linguistic sign represents a toponym (a specific kind of metonymy) based on the lexical sense of the linguistic sign referred to.</rdfs:comment>
    <rdfs:label xml:lang="en">uses as toponym</rdfs:label>
    <rdfs:label xml:lang="fr">utilise comme nom de lieu</rdfs:label>
    <rdfs:label xml:lang="de">verwendet als Personenname</rdfs:label>
</owl:ObjectProperty>

<!-- https://example.com/semshift#anthroponym -->

<owl:ObjectProperty rdf:about="https://https://example.com/semshift#anthroponym">
    <rdfs:domain rdf:resource="http://www.w3.org/ns/lemon/ontolex#LexicalSense"/>
    <rdfs:range  rdf:resource="http://www.w3.org/ns/lemon/ontolex#LexicalSense"/>
    <rdfs:subPropertyOf rdf:resource="http://www.w3.org/ns/lemon/vartrans#senseRel"/>
    <rdfs:comment xml:lang="en">The 'anthroponym' property indicates that the lexical sense of a linguistic sign represents an anthroponym (a specific kind of metonymy) based on the lexical sense of the linguistic sign referred to.</rdfs:comment>
    <rdfs:label xml:lang="en">uses as anthroponym</rdfs:label>
    <rdfs:label xml:lang="fr">utilise comme nom de personne</rdfs:label>
    <rdfs:label xml:lang="de">verwendet als Personenname</rdfs:label>
</owl:ObjectProperty>

<!-- https://example.com/semshift#minimalValue -->

<owl:ObjectProperty rdf:about="https://https://example.com/semshift#minimalValue">
    <rdfs:domain rdf:resource="http://www.w3.org/ns/lemon/ontolex#LexicalSense"/>
    <rdfs:range  rdf:resource="http://www.w3.org/ns/lemon/ontolex#LexicalSense"/>
    <rdfs:subPropertyOf rdf:resource="http://www.w3.org/ns/lemon/vartrans#senseRel"/>
    <rdfs:comment xml:lang="en">The 'minimalValue' property indicates that the lexical sense of a linguistic sign expresses a minimal value (a specific kind of metonymy) based on the lexical sense of the linguistic sign referred to.</rdfs:comment>
    <rdfs:label xml:lang="en">uses as minimal value</rdfs:label>
    <rdfs:label xml:lang="fr">utilise comme valeur minimale</rdfs:label>
    <rdfs:label xml:lang="de">verwendet als Minimalwert</rdfs:label>
</owl:ObjectProperty>

<!-- https://example.com/semshift#collective -->

<owl:ObjectProperty rdf:about="https://https://example.com/semshift#collective">
    <rdfs:domain rdf:resource="http://www.w3.org/ns/lemon/ontolex#LexicalSense"/>
    <rdfs:range  rdf:resource="http://www.w3.org/ns/lemon/ontolex#LexicalSense"/>
    <rdfs:subPropertyOf rdf:resource="http://www.w3.org/ns/lemon/vartrans#senseRel"/>
    <rdfs:comment xml:lang="en">The 'collective' property indicates that the lexical sense of a linguistic sign expresses a collective use (a specific kind of metonymy) of the lexical sense of the linguistic sign referred to.</rdfs:comment>
    <rdfs:label xml:lang="en">uses as collective value</rdfs:label>
    <rdfs:label xml:lang="fr">utilise dans un sens collectif</rdfs:label>
    <rdfs:label xml:lang="de">verwendet als Kollektivwert</rdfs:label>
</owl:ObjectProperty>

<!-- https://example.com/semshift#insult -->

<owl:ObjectProperty rdf:about="https://https://example.com/semshift#insult">
    <rdfs:domain rdf:resource="http://www.w3.org/ns/lemon/ontolex#LexicalSense"/>
    <rdfs:range  rdf:resource="http://www.w3.org/ns/lemon/ontolex#LexicalSense"/>
    <rdfs:subPropertyOf rdf:resource="http://www.w3.org/ns/lemon/vartrans#senseRel"/>
    <rdfs:comment xml:lang="en">The 'insult' property indicates that the lexical sense of a linguistic sign uses the lexical sense of the linguistic sign referred to as an insult (a specific kind of metonymy).</rdfs:comment>
    <rdfs:label xml:lang="en">uses as insult</rdfs:label>
    <rdfs:label xml:lang="fr">utilise comme insulte</rdfs:label>
    <rdfs:label xml:lang="de">verwendet als Beleidigung</rdfs:label>
</owl:ObjectProperty>

<!-- https://example.com/semshift#malediction -->

<owl:ObjectProperty rdf:about="https://https://example.com/semshift#malediction">
    <rdfs:domain rdf:resource="http://www.w3.org/ns/lemon/ontolex#LexicalSense"/>
    <rdfs:range  rdf:resource="http://www.w3.org/ns/lemon/ontolex#LexicalSense"/>
    <rdfs:subPropertyOf rdf:resource="http://www.w3.org/ns/lemon/vartrans#senseRel"/>
    <rdfs:comment xml:lang="en">The 'malediction' property indicates that the lexical sense of a linguistic sign uses the lexical sense of the linguistic sign referred to as a malediction (a specific kind of metonymy).</rdfs:comment>
    <rdfs:label xml:lang="en">uses as malediction</rdfs:label>
    <rdfs:label xml:lang="fr">utilise comme malédiction</rdfs:label>
    <rdfs:label xml:lang="de">verwendet als Fluchwort</rdfs:label>
</owl:ObjectProperty>

<!-- https://example.com/semshift#pejorative -->

<owl:ObjectProperty rdf:about="https://https://example.com/semshift#pejorative">
    <rdfs:domain rdf:resource="http://www.w3.org/ns/lemon/ontolex#LexicalSense"/>
    <rdfs:range  rdf:resource="http://www.w3.org/ns/lemon/ontolex#LexicalSense"/>
    <rdfs:subPropertyOf rdf:resource="http://www.w3.org/ns/lemon/vartrans#senseRel"/>
    <rdfs:comment xml:lang="en">The 'pejorative' property indicates that the lexical sense of a linguistic sign uses the lexical sense of the linguistic sign referred to in a pejorative way (a specific kind of metonymy).</rdfs:comment>
    <rdfs:label xml:lang="en">uses in a pejorative way</rdfs:label>
    <rdfs:label xml:lang="fr">utilise dans une manière péjorative</rdfs:label>
    <rdfs:label xml:lang="de">verwendet mit abwertender Bedeutung</rdfs:label>
</owl:ObjectProperty>

<!-- https://example.com/semshift#analogy -->

<owl:ObjectProperty rdf:about="https://https://example.com/semshift#analogy">
    <rdfs:domain rdf:resource="http://www.w3.org/ns/lemon/ontolex#LexicalSense"/>
    <rdfs:range  rdf:resource="http://www.w3.org/ns/lemon/ontolex#LexicalSense"/>
    <rdfs:subPropertyOf rdf:resource="http://www.w3.org/ns/lemon/vartrans#senseRel"/>
    <rdfs:comment xml:lang="en">The 'analogy' property indicates that the lexical sense of a linguistic sign expresses an analogy (a specific kind of metonymy) to the lexical sense of the linguistic sign referred to.</rdfs:comment>
    <rdfs:label xml:lang="en">uses in analogy with</rdfs:label>
    <rdfs:label xml:lang="fr">utilise par analogie avec</rdfs:label>
    <rdfs:label xml:lang="de">verwendet in Analogie zu</rdfs:label>
</owl:ObjectProperty>

<!-- https://example.com/semshift#extension -->

<owl:ObjectProperty rdf:about="https://https://example.com/semshift#extension">
    <rdfs:domain rdf:resource="http://www.w3.org/ns/lemon/ontolex#LexicalSense"/>
    <rdfs:range  rdf:resource="http://www.w3.org/ns/lemon/ontolex#LexicalSense"/>
    <rdfs:subPropertyOf rdf:resource="http://www.w3.org/ns/lemon/vartrans#senseRel"/>
    <owl:equivalentProperty>
        <owl:ObjectProperty rdf:about="http://www.lexinfo.net/ontology/3.0/lexinfo#hyperonym"/>
    </owl:equivalentProperty>
    <rdfs:comment xml:lang="en">The 'extension' property indicates that the sense of a linguistic sign represents a semantic extension of the sense of the linguistic sign referred to.</rdfs:comment>
    <rdfs:label xml:lang="en">is extension of</rdfs:label>
    <rdfs:label xml:lang="fr">est un élargissement de sens de</rdfs:label>
    <rdfs:label xml:lang="de">ist Bedeutungserweiterung von</rdfs:label>
    <rdfs:label xml:lang="de">ist Generalisierung von</rdfs:label>
    <rdfs:label xml:lang="de">ist Amplifikation von</rdfs:label>
</owl:ObjectProperty>

<!-- https://example.com/semshift#specification -->

<owl:ObjectProperty rdf:about="https://https://example.com/semshift#specification">
    <rdfs:domain rdf:resource="http://www.w3.org/ns/lemon/ontolex#LexicalSense"/>
    <rdfs:range  rdf:resource="http://www.w3.org/ns/lemon/ontolex#LexicalSense"/>
    <rdfs:subPropertyOf rdf:resource="http://www.w3.org/ns/lemon/vartrans#senseRel"/>
    <owl:equivalentProperty>
        <owl:ObjectProperty rdf:about="http://www.lexinfo.net/ontology/3.0/lexinfo#hyponym"/>
    </owl:equivalentProperty>
    <rdfs:comment xml:lang="en">The 'specification' property indicates that the sense of a linguistic sign represents a semantic specification of the sense of the linguistic sign referred to.</rdfs:comment>
    <rdfs:label xml:lang="en">is specification of</rdfs:label>
    <rdfs:label xml:lang="fr">est une spécification de</rdfs:label>
    <rdfs:label xml:lang="de">ist Bedeutungsverengung von</rdfs:label>
    <rdfs:label xml:lang="de">ist Spezialisierung von</rdfs:label>
</owl:ObjectProperty>

<!-- https://example.com/semshift#associativeRelation -->

<owl:ObjectProperty rdf:about="https://https://example.com/semshift#associativeRelation">
    <rdfs:domain rdf:resource="http://www.w3.org/ns/lemon/ontolex#LexicalSense"/>
    <rdfs:range>
      <owl:Class>
        <owl:unionOf rdf:parseType="Collection">
          <rdf:Description rdf:about="https://example.com/semshift#MetaphoricalSimilarity"/>
          <rdf:Description rdf:about="https://example.com/semshift#ConceptualContiguity"/>
          <rdf:Description rdf:about="https://example.com/semshift#TaxonomicSuperordination"/>
          <rdf:Description rdf:about="https://example.com/semshift#TaxonomicSubordination"/>
        </owl:unionOf>
      </owl:Class>
    </rdfs:range>
    <rdfs:comment xml:lang="en">The 'associativeRelation' property indicates the relation to an associative pattern underlying semantic shift.</rdfs:comment>
    <rdfs:label xml:lang="en">has an associative relation</rdfs:label>
    <rdfs:label xml:lang="fr">a une relation associative</rdfs:label>
    <rdfs:label xml:lang="de">hat die Assoziationsrelation</rdfs:label>
</owl:ObjectProperty>

<!--
///////////////////////////////////////////////////////////////////////////////////////
//
// Classes
//
///////////////////////////////////////////////////////////////////////////////////////
 -->

<!-- https://example.com/semshift#MetaphoricalSimilarity -->

<owl:Class rdf:about="https://example.com/semshift#MetaphoricalSimilarity">
    <rdfs:subClassOf rdf:resource="https://example.com/semshift#AssociativeRelation"/>
    <rdfs:comment xml:lang="en">This is the associative relation of metaphorical similarity.</rdfs:comment>
    <rdfs:label   xml:lang="en">metaphorical similarity</rdfs:label>
    <rdfs:label   xml:lang="fr">similarité métaphorique</rdfs:label>
    <rdfs:label   xml:lang="de">metaphorische Similarität</rdfs:label>
</owl:Class>

<!-- https://example.com/semshift#ConceptualContiguity -->

<owl:Class rdf:about="https://example.com/semshift#ConceptualContiguity">
    <rdfs:subClassOf rdf:resource="https://example.com/semshift#AssociativeRelation"/>
    <rdfs:comment xml:lang="en">This is the associative relation of conceptual contiguity.</rdfs:comment>
    <rdfs:label   xml:lang="en">conceptual contiguity</rdfs:label>
    <rdfs:label   xml:lang="fr">contigüité conceptionnelle</rdfs:label>
    <rdfs:label   xml:lang="de">konzeptionelle Kontiguität</rdfs:label>
</owl:Class>

<!-- https://example.com/semshift#TaxonomicSuperordination -->

<owl:Class rdf:about="https://example.com/semshift#TaxonomicSuperordination">
    <rdfs:subClassOf rdf:resource="https://example.com/semshift#AssociativeRelation"/>
    <rdfs:comment xml:lang="en">This is the associative relation of taxonomic superordination.</rdfs:comment>
    <rdfs:label   xml:lang="en">taxonomic superordination</rdfs:label>
    <rdfs:label   xml:lang="fr">superordination taxonomique</rdfs:label>
    <rdfs:label   xml:lang="de">taxonomische Überordnung</rdfs:label>
</owl:Class>

<!-- https://example.com/semshift#TaxonomicSubordination -->

<owl:Class rdf:about="https://example.com/semshift#TaxonomicSubordination">
    <rdfs:subClassOf rdf:resource="https://example.com/semshift#AssociativeRelation"/>
    <rdfs:comment xml:lang="en">This is the associative relation of taxonomic subordination.</rdfs:comment>
    <rdfs:label   xml:lang="en">taxonomic subordination</rdfs:label>
    <rdfs:label   xml:lang="fr">subordination taxonomique</rdfs:label>
    <rdfs:label   xml:lang="de">taxonomische Unterordnung</rdfs:label>
</owl:Class>

</rdf:RDF>
